kk

examples/n_german/nMutual1.thy
@@ -5,7 +5,7 @@ begin
 
 subsection \<open>Definitions\<close>
 
-text \<open>Represents the four states: idle, try, critical, exit\<close>
+text \<open>type definitions Represents the four states: idle, try, critical, exit\<close>
 
 definition I :: scalrValueType where [simp]: "I \<equiv> enum ''control'' ''I''"
 definition T :: scalrValueType where [simp]: "T \<equiv> enum ''control'' ''T''"
@@ -15,7 +15,7 @@ definition E :: scalrValueType where [simp]: "E \<equiv> enum ''control'' ''E''"
 definition true :: scalrValueType where [simp]: "true \<equiv> boolV True"
 definition false :: scalrValueType where [simp]: "false \<equiv> boolV False"
 
-text \<open>Initial condition: all processes in idle.
+text \<open>initial state Initial condition: all processes in idle.
   \<forall>i. n[i] = I
 \<close>
 definition initSpec0 :: "nat \<Rightarrow> formula" where
@@ -27,25 +27,53 @@ text \<open>Initial condition: x is True
 definition initSpec1 :: formula where
   "initSpec1 \<equiv> IVar (Ident ''x'') =\<^sub>f Const true"
 
-text \<open>There cannot be one state in exit and another in critical or exit.
-  n[i] = E \<longrightarrow> (\<forall>j. i \<noteq> j \<longrightarrow> n[j] \<noteq> C \<and> n[j] \<noteq> E)
-\<close>
-definition invAux :: "nat \<Rightarrow> nat \<Rightarrow> formula" where
-  "invAux N i \<equiv> IVar (Para ''n'' i) =\<^sub>f Const E \<longrightarrow>\<^sub>f forallFormExcl 
-    (\<lambda>j. \<not>\<^sub>f IVar (Para ''n'' j) =\<^sub>f Const C \<and>\<^sub>f \<not>\<^sub>f IVar (Para ''n'' j) =\<^sub>f Const E) i N"  
 
-text \<open>Try enter critical region
-  n[i] = I \<rightarrow> n[i] := T
-\<close>
+
+definition allInitSpecs :: "nat \<Rightarrow> formula list" where
+  "allInitSpecs N \<equiv> [
+    (initSpec0 N),
+    (initSpec1 ) 
+  ]"
+
+
+lemma symPreds:
+  "symPredSet' N ({initSpec0 N} \<union> {initSpec1})"
+  apply (rule symPredsUnion)
+  subgoal
+    unfolding initSpec0_def
+    apply (rule symPredSetForall)
+    unfolding symParamForm_def by auto    
+  subgoal
+    unfolding symPredSet'_def initSpec1_def by auto
+  done
+
+
+lemma symPreds':
+  "symPredSet' N (set (allInitSpecs N))"
+  proof -
+    have b1:"(set (allInitSpecs N)) =
+      {(initSpec0 N)} \<union>
+    {initSpec1}" (is "?LHS=?RHS")
+      using allInitSpecs_def by auto
+    have b2:"symPredSet' N ?RHS"
+      using symPreds by blast
+    show "symPredSet' N (set (allInitSpecs N))"
+      using b1 b2 by auto  
+  qed    
+
+ 
+
+text \<open>rules \<close>
+
+ 
+
 definition n_Try :: "nat \<Rightarrow> rule" where
   "n_Try i \<equiv>
     IVar (Para ''n'' i) =\<^sub>f Const I
    \<triangleright>
     assign (Para ''n'' i, Const T)"
 
-text \<open>Enter critical region
-  n[i] = T \<and> x = True \<rightarrow> n[i] := C; x := False
-\<close>
+ 
 definition n_Crit :: "nat \<Rightarrow> rule" where
   "n_Crit i \<equiv>
     IVar (Para ''n'' i) =\<^sub>f Const T \<and>\<^sub>f
@@ -54,18 +82,14 @@ definition n_Crit :: "nat \<Rightarrow> rule" where
     assign (Para ''n'' i, Const C) ||
     assign (Ident ''x'', Const false)"
 
-text \<open>Exit critical region
-  n[i] = C \<rightarrow> n[i] := E
-\<close>
+ 
 definition n_Exit :: "nat \<Rightarrow> rule" where
   "n_Exit i \<equiv>
     IVar (Para ''n'' i) =\<^sub>f Const C
    \<triangleright>
     assign (Para ''n'' i, Const E)"
 
-text \<open>Move to idle
-  n[i] = E \<rightarrow> n[i] := I; x := True
-\<close>
+ 
 definition n_Idle :: "nat \<Rightarrow> rule" where
   "n_Idle i \<equiv>
     IVar (Para ''n'' i) =\<^sub>f Const E
@@ -101,11 +125,6 @@ lemma absInitSpec:
         "absTransfForm M initSpec1 = initSpec1"
   unfolding initSpec0_def initSpec1_def using assms by auto
 
-lemma symInvAux:
-  "symParamForm N (invAux N)"
-  unfolding invAux_def
-  apply (auto intro!: symParamFormImply symParamFormAnd symParamFormForall symParamFormForallExcl)
-  unfolding symParamForm_def symParamForm2_def equivForm_def by auto
 
 lemma symTry:
   "symParamRule N n_Try"
@@ -131,6 +150,20 @@ lemma symIdle:
   "absTransfRule M (n_Idle i) = (if i \<le> M then n_Idle i else n_Idle_abs1)"
   unfolding n_Idle_def n_Idle_abs1_def symParamRule_def by auto
 
+text \<open>aux invs\<close>
+
+definition invAux :: "nat \<Rightarrow> nat \<Rightarrow> formula" where
+  "invAux N i \<equiv> IVar (Para ''n'' i) =\<^sub>f Const E \<longrightarrow>\<^sub>f forallFormExcl 
+    (\<lambda>j. \<not>\<^sub>f IVar (Para ''n'' j) =\<^sub>f Const C \<and>\<^sub>f \<not>\<^sub>f IVar (Para ''n'' j) =\<^sub>f Const E) i N"  
+
+
+lemma symInvAux:
+  "symParamForm N (invAux N)"
+  unfolding invAux_def
+  apply (auto intro!: symParamFormImply symParamFormAnd symParamFormForall symParamFormForallExcl)
+  unfolding symParamForm_def symParamForm2_def equivForm_def by auto
+
+
 text \<open>Move to idle, strengthened:
   n[i] = E \<and>
   (\<forall>j. i \<noteq> j \<longrightarrow> n[j] \<noteq> C) \<and>
@@ -149,19 +182,17 @@ lemma n_Idle2Eq:
   "strengthenRule2 (invAux N i) (n_Idle i) = n_Idle2_ref N i"
   by (auto simp add: strengthenRule2.simps invAux_def n_Idle_def n_Idle2_ref_def)
 
-lemma wellFormedIdle2:
+lemma symIdle2_ref:
   "symParamRule N (n_Idle2_ref N)"
   "wellFormedRule N (n_Idle2_ref N i)"
+  "M \<le> N \<Longrightarrow> absTransfRule M (n_Idle2_ref N i) = (if i \<le> M then n_Idle i else n_Idle_abs2 M)"
   unfolding n_Idle2_ref_def
    apply (auto intro!: symParamRuleI symParamFormAnd symParamFormForallExcl)
-  unfolding symParamForm_def symParamForm2_def symParamStatement_def by auto
-
-lemma absIdle2:
-  "M \<le> N \<Longrightarrow> absTransfRule M (n_Idle2_ref N i) = (if i \<le> M then n_Idle i else n_Idle_abs2 M)"
-  unfolding n_Idle_def n_Idle_abs2_def n_Idle2_ref_def by auto
+  unfolding symParamForm_def symParamForm2_def symParamStatement_def apply auto[1]
+   unfolding n_Idle_def n_Idle_abs2_def n_Idle2_ref_def by auto 
 
 
-subsection \<open>Putting everything together\<close>
+subsection \<open>Putting everything together ---definition of rules\<close>
 
 definition n_Trys :: "nat \<Rightarrow> rule set" where
   "n_Trys N \<equiv> oneParamCons N n_Try"
@@ -198,7 +229,9 @@ lemma rulesSym':
   "symProtRules' N (rules' N)"
   unfolding rules'_def apply (intro symProtRulesUnion)
   using n_CritsIsSym n_ExitsIsSym n_IdlesIsSym n_TrysIsSym by auto
- 
+
+text \<open>strengthened rules with auxiliary invariants\<close>
+
 definition pair1 :: "(nat \<Rightarrow> formula) \<times> (nat \<Rightarrow> formula)" where
   "pair1 \<equiv> (\<lambda>i. IVar (Para ''n'' i) =\<^sub>f Const E,
             \<lambda>j. \<not>\<^sub>f IVar (Para ''n'' j) =\<^sub>f Const C \<and>\<^sub>f \<not>\<^sub>f IVar (Para ''n'' j) =\<^sub>f Const E)"
@@ -218,7 +251,7 @@ lemma n_Idle2sIsSym:
   "symProtRules' N (n_Idle2s N)"
   unfolding n_Idle2s_def
   apply (rule symParaRuleInfSymRuleSet)
-  using invAux_def n_Idle2Eq wellFormedIdle2(1) constrInvByExcl_def
+  using invAux_def n_Idle2Eq symIdle2_ref(1) constrInvByExcl_def
   by (auto simp add: pair1_def)
  
 lemma rule2'IsSym:
@@ -227,15 +260,18 @@ lemma rule2'IsSym:
   apply (intro symProtRulesUnion)
   using n_CritsIsSym n_ExitsIsSym n_Idle2sIsSym n_TrysIsSym by auto 
 
+text \<open>type value information on variables occurring in aux(0,1)\<close>
+
 definition type_inv :: "nat \<Rightarrow> state \<Rightarrow> bool" where
   "type_inv N s = (\<forall>i. i \<le> N \<longrightarrow> s (Para ''n'' i) = I \<or> s (Para ''n'' i) = T \<or> s (Para ''n'' i) = C \<or> s (Para ''n'' i) = E)"
 
+thm strengthenRule2.simps
 lemma invOnStateOfN' [simp,intro]:
-  assumes "reachableUpTo ({initSpec0 N} \<union> {initSpec1}) (rules2' N) k s"
+  assumes "reachableUpTo (set (allInitSpecs N)) (rules2' N) k s"
   shows "type_inv N s"
   apply (rule invIntro[OF _ _ assms])
   subgoal for s
-    by (auto simp add: type_inv_def initSpec0_def)
+    by (auto simp add: allInitSpecs_def type_inv_def initSpec0_def)
   subgoal for r sk
     unfolding rules2'_def apply auto
     subgoal unfolding n_Trys_def apply auto unfolding type_inv_def n_Try_def by auto
@@ -247,34 +283,11 @@ lemma invOnStateOfN' [simp,intro]:
 
 lemma invOnStateOfN'' [simp,intro]:
   assumes a: "reachableUpTo fs rs k s"
-  shows "fs = {initSpec0 N} \<union> {initSpec1} \<longrightarrow> rs = rules2' N \<longrightarrow> i \<le> N \<longrightarrow> isEnumVal s (Para ''n'' i)"
+  shows "fs = (set (allInitSpecs N)) \<longrightarrow> rs = rules2' N \<longrightarrow> i \<le> N \<longrightarrow> isEnumVal s (Para ''n'' i)"
   using invOnStateOfN' unfolding type_inv_def C_def E_def I_def T_def
   by (metis assms getValueType.simps(1) isEnumVal_def typeOf_def)
 
-lemma symPreds:
-  "symPredSet' N ({initSpec0 N} \<union> {initSpec1})"
-  apply (rule symPredsUnion)
-  subgoal
-    unfolding initSpec0_def
-    apply (rule symPredSetForall)
-    unfolding symParamForm_def by auto    
-  subgoal
-    unfolding symPredSet'_def initSpec1_def by auto
-  done
-
-definition absTransfRuleSet :: "nat \<Rightarrow> rule set \<Rightarrow> rule set" where
-  "absTransfRuleSet M rs = absTransfRule M ` rs"
-
-lemma absGen:
-  assumes "\<And>i. absTransfRule M (f i) = (if i \<le> M then g i else h)"
-    and "M < N"
-  shows "absTransfRule M ` (oneParamCons N f) = (oneParamCons M g) \<union> {h}"
-  apply (auto simp add: assms image_def)
-   apply (rule exI[where x="f (M + 1)"])
-  apply (metis add_le_same_cancel1 assms(1) assms(2) discrete not_one_le_zero)
-  subgoal for i apply (rule exI[where x="f i"])
-    by (metis assms(1) assms(2) le_trans nat_le_linear not_le)
-  done
+text\<open>abstract rules\<close>
 
 lemma absTrys:
   "M < N \<Longrightarrow> absTransfRule M ` (n_Trys N) = (n_Trys M) \<union> {chaos \<triangleright> skip}"
@@ -296,7 +309,7 @@ lemma n_Idle2_ref':
 lemma absIdle2s:
   "M < N \<Longrightarrow> absTransfRule M ` (n_Idle2s N) = (n_Idles M) \<union> {n_Idle_abs2 M}"
   unfolding n_Idle2s_def n_Idles_def n_Idle2_ref'
-  apply (rule absGen) using absIdle2 by auto
+  apply (rule absGen) using symIdle2_ref(3) by auto
 
 definition absRules :: "nat \<Rightarrow> rule set" where
   "absRules M \<equiv> n_Trys M \<union> n_Exits M \<union> n_Crits M \<union> n_Idles M \<union>
@@ -314,11 +327,11 @@ lemma absProtSim:
     and a3: "M = 1"
     and a4: "\<forall>i f s.
        f \<in> F \<longrightarrow>
-       reachableUpTo {f'. \<exists>f. f \<in> {initSpec0 N} \<union> {initSpec1} \<and> f' = absTransfForm M f}
+       reachableUpTo {f'. \<exists>f. f \<in> (set (allInitSpecs N)) \<and> f' = absTransfForm M f}
         (absRules M) i s \<longrightarrow>
        formEval (constrInv f 0 1) s"
   shows "\<forall>f s. f \<in> constrInvByExcls F N \<longrightarrow> 
-    reachableUpTo ({initSpec0 N} \<union> {initSpec1}) (rules' N) i s \<longrightarrow> formEval f s"
+    reachableUpTo (set (allInitSpecs N)) (rules' N) i s \<longrightarrow> formEval f s"
 proof (rule_tac ?rs2.0="rules2' N" in CMP)
   show "\<And>r. r \<in> rules' N \<longrightarrow> wellFormedRule N r"
     by (auto simp add: rules'_def n_Trys_def symTry(2) n_Crits_def symCrit(2)
@@ -330,13 +343,13 @@ next
   show "symProtRules' N (rules' N)"
     using rulesSym' by blast
 next
-  show "symPredSet' N ({initSpec0 N} \<union> {initSpec1})"
-    using symPreds by blast
+  show "symPredSet' N (set (allInitSpecs N))"
+    using symPreds' by blast
 next
   show "M \<le> N"
     using a2 by arith
 next
-  show "\<forall>s i f. reachableUpTo ({initSpec0 N} \<union> {initSpec1}) (rules2' N) i s \<longrightarrow>
+  show "\<forall>s i f. reachableUpTo (set (allInitSpecs N)) (rules2' N) i s \<longrightarrow>
         f \<in> F \<longrightarrow> (\<forall>v. v \<in> varOfForm (constrInv f 0 1) \<longrightarrow> s v = abs1 M s v)"
     using invOnStateOfN'' enumValAbsRemainSame
     unfolding F_def pair1_def using a2 a3 by auto
@@ -350,7 +363,8 @@ next
       using that apply (auto simp add: n_Idle2s_def)
       subgoal for i
         apply (rule exI[where x="n_Idle i"])
-        unfolding F_def pair1_def by (auto simp add: constrInvByExcl_def strengthenRule2.simps n_Idle_def rules'_def n_Idles_def)
+        unfolding F_def pair1_def 
+        by (auto simp add: constrInvByExcl_def strengthenRule2.simps n_Idle_def rules'_def n_Idles_def)
       done
     then show ?thesis
       apply (unfold rules2'_def rules'_def) by auto
@@ -362,7 +376,8 @@ next
   show "\<forall>r. r \<in> rules' N \<longrightarrow>
     (\<exists>f. f \<in> constrInvByExcls F N \<and> strengthenRule2 f r \<in> rules2' N) \<or> r \<in> rules2' N"
   proof -
-    have "\<exists>f. f \<in> constrInvByExcls F N \<and> strengthenRule2 f r \<in> n_Trys N \<union> n_Crits N \<union> n_Exits N \<union> n_Idle2s N"
+    have "\<exists>f. f \<in> constrInvByExcls F N \<and> 
+    strengthenRule2 f r \<in> n_Trys N \<union> n_Crits N \<union> n_Exits N \<union> n_Idle2s N"
       if "r \<in> n_Idles N" for r
       using that apply (auto simp add: n_Idles_def)
       subgoal for i
